move old files to old/, rename files properly, add P-HMAC spec with ipad/opad, get H-HMAC to recompile. TODO: fill in the ipad/opad relation (figure out a simpler way)

HMAC_spec_harvard.v
@@ -1,11 +1,10 @@
 Set Implicit Arguments.
 
-
 Require Import Bvector.
 Require Import List.
 Require Import Arith.
 
-Require Import HMAC_functional_prog_new.
+Require Import HMAC_functional_prog.
 Require Import Integers.
 Require Import Coqlib.
 
@@ -29,31 +28,34 @@ SearchAbout Bvector.
 Print Bvector.
 Check Bvector 10.
 Check [true]. 
+Print Vector.
 
+(* b = block size
+   c = digest (output) size
+   p = padding = b - c (fixed) *)
   Variable c p : nat.
-  (* b is block size, c is digest (output) size, p is padding *)
   Definition b := (c + p)%nat.
-  Check b.
   
   (* The compression function *)
-  (* hash_blocks: registers -> block -> registers *)
   Variable h : Bvector c -> Bvector b -> Bvector c.
   (* The initialization vector is part of the spec of the hash function. *)
-  (* TODO: is the IV standardized in the spec? does it need to have certain properties for
-   the proof? *)
   Variable iv : Bvector c.
   (* The iteration of the compression function gives a keyed hash function on lists of words. *)
   Definition h_star k (m : list (Bvector b)) :=
     fold_left h m k.
   (* The composition of the keyed hash function with the IV gives a hash function on lists of words. *)
-  (* TODO check how this corresponds to SHA *)
   Definition hash_words := h_star iv.
-Check hash_words.
-Check h_star.
+
+  (* TODO check how this corresponds to SHA
+     Seems that h = SHA compression function
+     hash_words with SHA's iv is SHA
+   *)
+  Check hash_words.
+  Check h_star.
 
   Variable splitAndPad : Blist -> list (Bvector b).
 
-  (* TODO examine this hypothesis *)
+  (* TODO examine this hypothesis, prove that MD lemmas imply it *)
   Hypothesis splitAndPad_1_1 : 
     forall b1 b2,
       splitAndPad b1 = splitAndPad b2 ->
@@ -78,169 +80,40 @@ Check h_star.
       let h_in := (hash_words (k_In :: m)) in 
         hash_words (k_Out :: (app_fpad h_in) :: nil).
   
-  (* b + b comes from ( *)
   Definition HMAC_2K (k : Bvector (b + b)) (m : Blist) :=
     GHMAC_2K k (splitAndPad m).
 
 Check HMAC_2K.
 (* HMAC_2K
      : Bvector (b + b) -> Blist -> Bvector c *)
-SearchAbout Bvector.
-(* Bvector (b + b) -> Blist -> BVector c *)
 
-Print splitVector.
-
-Theorem test : forall (k : Bvector (b + b)) (m : Blist),
-  HMAC_2K k m = HMAC_2K k m.
-Proof.
-  intros k m.
-  unfold HMAC_2K.               (* splitAndPad is abstract *)
-  unfold GHMAC_2K.
-  unfold hash_words.
-  unfold h_star. 
-  (* unfold splitVector. *)
-Abort.
-
-Print Bvector.                  (* Vector.t bool : nat -> Set *)
-(* Check [true]%(Bvector 1). *)
-(* Cannot compute since Variables are not instantiated  -- TODO, how to instantiate 
-(e.g. with SHA256? does it have the right type? 
-SHA256 : list Z -> list Z *)
-(* Eval compute in HMAC_2K [true; true] [false]. *)
-
-  (* opad and ipad are constants defined in the HMAC spec. *)
-  Variable opad ipad : Bvector b. (* c + p *)
-  Definition GHMAC (k : Bvector b) :=
-    GHMAC_2K (Vector.append (BVxor _ k opad) (BVxor _ k ipad)).
+(* opad and ipad are constants defined in the HMAC spec. *)
+Variable opad ipad : Bvector b.
+Definition GHMAC (k : Bvector b) :=
+  GHMAC_2K (Vector.append (BVxor _ k opad) (BVxor _ k ipad)).
 
 Print BVxor.
 
-  (* Doesn't seem to take into account the hash function's input block size (see mkKey in P. spec) *)
-  Definition HMAC (k : Bvector b) :=
-    HMAC_2K (Vector.append (BVxor _ k opad) (BVxor _ k ipad)).
+
+Definition HMAC (k : Bvector b) :=
+  HMAC_2K (Vector.append (BVxor _ k opad) (BVxor _ k ipad)).
 
 Check HMAC.                     (*  : Bvector b -> Blist -> Bvector c *)
 
-  (* Bvector or Blist? *)
-Check HMAC_2K.                  (* TODO confirm that this is actually the right version *)
-
 End HMAC.
 
-(* -------------- *)
+(* ----------------------------------------------------------- Theorem definitions *)
 
-Require Import HMAC_functional_prog_2.
+Check HMAC_SHA256.HMAC.            (* list Z -> list Z -> list Z *)
 
-(* How to get the other HMAC? *)
-(* TODO: compile HMAC_functional_prog_2 *)
-Check HMAC_FUN.HMAC.            (* list Z -> list Z -> list Z *)
-
-(* Bvector (plus c p)  *)
-
-(* relationship between a list Z (of bytes) and a Bvector of size (c + p):
-toBvector (bytes_to_bits k) = K?
-(don't actually need the Bvector, just c + p, or its length) <-- deprecated,
-want equality
- *)
-Inductive bytes_bits_vector (c p : nat) (k : list Z) : Bvector (plus c p) -> Prop :=
-  | test_n : forall (K : Bvector (plus c p)), bytes_bits_vector c p k K (* ?? TODO *)
-.
-
-(* relating list Z to Blist
-bytes_to_bits m = length M
-
-TODO: big-endian, little-endian?
-*)
-Inductive bytes_bits_lists (m : list Z) : Blist -> Prop :=
-  | test_n' : forall M : Blist, bytes_bits_lists m M
-.
-
-(* the hashes are "the same": list Z vs Bvector c
-
-toBvector (bytes_to_bits h) = H
-this is *almost* the same as bytes_bits_vector, except just c, not c + p
- *)
-Inductive bytes_bits_vector' (c : nat) (h : list Z) : Bvector c -> Prop :=
-  | test_n'' : forall (H : Bvector c), bytes_bits_vector' h H
-.
-(* TODO: compare to rel1. How do dependent types and inductive props work? *)
-
-
-
-(* TODO:
-Definition convertByteBits (b: byte) (B: Bvector 8): Prop :=
-  exists b0, ... b7 (*all of type bool*),
-   B = [b0, b1, ... b7] /\
-   b = (asZ b0) + 2 * (asZ b1) * 4 * (asZ b2) + .. + 128 * (asZ b7).
-
-where Definition asZ (x:bool):Z := if x then 1 else 0.
-*)
-
-Check bytes_bits_vector.
-Check HMAC_FUN.HMAC.
-Check HMAC_SHA256.HMAC.         (* ? *)
-Check HMAC.
-(* HMAC
-     : forall c p : nat,
-       (Bvector c -> Bvector (b c p) -> Bvector c) ->   // compression function h
-       Bvector c ->                          // iv, h's initialization vector
-       (Blist -> list (Bvector (b c p))) ->  // splitAndPad (e.g. generate_and_pad)
-       Bvector p ->                          // fpad, constant-length padding
-       Bvector (b c p) ->                    // opad
-       Bvector (b c p) ->                    // ipad
-
-^ Note: this has to do with the internals of SHA256 and HMAC too
-SHA's compression function, iv, generate_and_pad (with block vectors),
-HMAC's key padding function, HMAC's opad and ipad
-
-How to convert?
-
-Bvector (b c p) -> Blist -> Bvector c        // key, message, outputted hash
-k is of length b
-b = block size
-c = output size
-c + p = output size padded to block size
-
-why pad the key? why not just let it be size b?
- *)
-
-(* Is this the theorem we want? Is it useful for the rest of the proofs?
-Should it be more abstract? 
-
-also, no key padding
-add assumption that the key is padded to the right length (b)
-password of length b
-modify?
-*)
-
-Print Blist.
-
-(* maybe bvector of length 8, convert to Blist later? 
-TODO big-endian vs. little-endian *)
-(* Parameter byte_to_bits : Z -> Bvector 8. *)
-  (* Vector.nil bool. TODO *)
-SearchAbout Vector.t.
-
-(* Bvector is little-endian (least significant bit at head; list Z are just translated
+  (* Bvector is little-endian (least significant bit at head; list Z are just translated
 from the string (ascii -> nat -> Z); but Int are packed big-endian (with 4 Z -> 1 Int)
 
-each Z is one byte (8 bits) *
+each Z is one byte (8 bits) *)
 
-bytes -> bits is ok
-bits -> bytes is not ok
-*)
-(*
-Don't have an assurance that 0 <= byte < 256 
-TODO: add isbyteZ (from SHA256.v), 0 <= i <= 256 
+(* TODO: add isbyteZ (from SHA256.v), 0 <= i <= 256 *)
 
-1 2 3 4 5 6 7 8
-*)
-
-SearchAbout Z.
-Eval compute in zle 5 10.
-Check zle.
-Check zle_true.
-SearchAbout nat.
-Check N.
+(* *************** byte/bit computational *)
 
 (* TODO: finish this
 
@@ -248,8 +121,7 @@ The term "Vector.append (iterate n' num_new) [bool_digit]" has type
  "Vector.t bool (n' + 1)" while it is expected to have type 
 "Bvector (S n')".
 
-Function with proof of equivalence? see hash_blocks
- *)
+Function with proof of equivalence? see hash_blocks  *)
 
 (*
 Fixpoint iterate (n : nat) (byte : nat) : Bvector n :=
@@ -262,14 +134,9 @@ Fixpoint iterate (n : nat) (byte : nat) : Bvector n :=
       Vector.append (iterate n' num_new) [bool_digit] (* could reverse instead *)
   end.
 
-(* reverse? 
-0 <= byte < 256, integer 
-
-[0, 1, 2, 3, 4, 5, 6, 7] <-- bool
-*)
 Fixpoint byte_to_bits (byte : Z) : Bvector 8 :=
   let max_pow_two := 7 in
-  iterate (max_pow_two + 1) (nat_of_Z byte).    (* or iterate 8? *)
+  iterate (max_pow_two + 1) (nat_of_Z byte).
 *)
 
 Parameter byte_to_bits : Z -> Bvector 8.
@@ -287,77 +154,204 @@ Fixpoint bytes_to_bits (bytes : list Z) : Bvector (length bytes * 8) :=
     | x :: xs => Vector.append (byte_to_bits x) (bytes_to_bits xs)
   end.
 
-(* -------------------------------- *)
+(* ************* inductive defs *)
+  
+SearchAbout Bvector.
 
-Parameter sha_iv : Bvector (8 * SHA256_.DigestLength).
+Definition asZ (x : bool) : Z := if x then 1 else 0.
+
+(* TODO: maybe prefer b : byte, with Byte.repr? *)
+Definition convertByteBits (b : Z) (B : Bvector 8) : Prop :=
+  exists (b0 b1 b2 b3 b4 b5 b6 b7 : bool),
+   B = [b0; b1; b2; b3; b4; b5; b6; b7] /\
+   b =  (1 * (asZ b0) + 2 * (asZ b1) + 4 * (asZ b2) + 8 * (asZ b3)
+         + 16 * (asZ b4) + 32 * (asZ b5) + 64 * (asZ b6) + 128 * (asZ b7)).
+
+(* *** *)
+
+(* relationship between a list Z (of bytes) and a Bvector of size (c + p):
+toBvector (bytes_to_bits k) = K?
+
+This definition is not easy to use; replaced with bytes_bits_vector' in theorem
+ *)
+Inductive bytes_bits_vector (c p : nat) (k : list Z) : Bvector (plus c p) -> Prop :=
+  | test_n : forall (K : Bvector (plus c p)),
+               bytes_bits_vector c p k K (* TODO *)
+.
+
+(* relating list Z to Blist
+bytes_to_bits m = length M
+
+TODO: big-endian, little-endian?
+*)
+Inductive bytes_bits_lists : list Z -> Blist -> Prop :=
+  | eq_empty : bytes_bits_lists nil nil
+  | eq_cons : forall (bytes : list Z) (bits : Blist)
+                     (byte : Z) (b0 b1 b2 b3 b4 b5 b6 b7 : bool),
+                bytes_bits_lists bytes bits ->
+                convertByteBits byte ([b0; b1; b2; b3; b4; b5; b6; b7]) ->
+                bytes_bits_lists (byte :: bytes)
+                                (b0 :: b1 :: b2 :: b3 :: b4 :: b5 :: b6 :: b7 :: bits)
+.
+
+(* the hashes are "the same": list Z vs Bvector c
+
+toBvector (bytes_to_bits h) = H
+this is *almost* the same as bytes_bits_vector, except just c, not c + p
+ *)
+(* note: need to name c in order to use in Bvector c -- but then need to use names *)
+Inductive bytes_bits_vector' (len : nat) (bytes : list Z) (bits : Bvector len) : Prop :=
+  | eq_empty_v : bytes = nil -> len = 0%nat -> bytes_bits_vector' bytes bits
+  (* remove -> from eq_empty_v TODO *)
+  | eq_cons_v : bytes_bits_vector' bytes bits
+      (* forall (len' : nat) (bytes' : list Z) (bits' : Bvector len)
+                       (byte : Z) (b0 b1 b2 b3 b4 b5 b6 b7 : bool),
+                  bytes_bits_vector' bytes' bits' ->
+                  convertByteBits byte ([b0; b1; b2; b3; b4; b5; b6; b7]) ->
+                  bytes_bits_vector' (byte :: bytes')
+                                   (b0 :: b1 :: b2 :: b3 :: b4 :: b5 :: b6 :: b7 :: bits')
+      *) (* TODO *)
+.
+(* TODO: compare to rel1. How do dependent types and inductive props work? *)
+
+Check bytes_bits_vector.
+Check HMAC_SHA256.HMAC.         (* ? *)
+Check HMAC.
+(* HMAC
+     : forall c p : nat,
+       (Bvector c -> Bvector (b c p) -> Bvector c) ->   // compression function h
+       Bvector c ->                          // iv, h's initialization vector
+       (Blist -> list (Bvector (b c p))) ->  // splitAndPad (e.g. generate_and_pad)
+       Bvector p ->                          // fpad, constant-length padding
+       Bvector (b c p) ->                    // opad
+       Bvector (b c p) ->                    // ipad
+
+^ Note: this has to do with the internals of SHA256 and HMAC too
+SHA's compression function, iv, generate_and_pad (with block vectors),
+HMAC's key padding function, HMAC's opad and ipad.
+How to convert?
+
+       Bvector (b c p) -> Blist -> Bvector c        // key, message, outputted hash
+
+k is of length b
+b = block size
+c = output size
+p = padding = b - c
+
+why pad the key? why not just let it be size b?
+ *)
+
+(* ----------------------------------------- Theorem and parameters *)
+
+Parameter sha_iv : Bvector (SHA256_.DigestLength * 8).
 
 (* Definition sha_h : list Z -> list Z := SHA256_.Hash. *)
-Parameter sha_h : forall (c p : nat) (b:nat -> nat -> nat),
-                    Bvector c -> Bvector (b c p) -> Bvector c.
-(* due to implicit parameters, only requires c or p, and b *)
+(* TODO: c = 32, p = 32 *)
+Parameter sha_h : forall (c p : nat) (b:nat -> nat -> nat), Bvector c -> Bvector (b c p) -> Bvector c.
 
-(* corresponds to block size, b = plus *)
+(* corresponds to block size. b = plus *)
 
 (* TODO: email adam about fpad: it's not padding the key *)
 
 (*  "Blist -> list (Bvector (b SHA256_.DigestLength c))" *)
 Parameter sha_splitandpad_vector :
-  forall (p : nat), Blist -> list (Bvector ((SHA256_.DigestLength * 8) + p)).
+  forall (p: nat), Blist -> list (Bvector (SHA256_.DigestLength * 8 + p)).
 
 Parameter fpad : forall (p : nat), Bvector p.
 
 (* want Bvector b = 512 bits *)
 Print Byte.int.
 Print Byte.repr.
-Check HMAC_SHA256.sixtyfour HMAC_SHA256.Opad.
 Check Byte.unsigned.
-Definition opad := bytes_to_bits
+Check HMAC_SHA256.sixtyfour.
+(*
+Definition opad := 
+     bytes_to_bits
                      (map Byte.unsigned (HMAC_SHA256.sixtyfour HMAC_SHA256.Opad)).
+Check opad. 
 Definition ipad := bytes_to_bits
                      (map Byte.unsigned (HMAC_SHA256.sixtyfour HMAC_SHA256.Ipad)).
+*)
 
-Check HMAC.
+(*
+TODO: 8/20/14
 
-(* 
-Email Adam about fpad
+Key is not being padded? Need to assume the padded key is of length b
+Email Adam about fpad: it's not used to pad the key
 Figure out what parameters are
 Fill in the relations
-Byte to bits
 
-New theorem
-Parametrize C HMAC by OPAD and IPAD + they need to be different in at least one bit
-   (does adam need this?)
+Byte to bits: computational vs. prop
+  bytes_bits_vector: problem
+  bytes_to_bits: 2 problems
+  still need the computational version for opad?
 
-Now, write individual functions (e.g. sha_h, which is still abstract)
-and prove them equivalent? different types....
+Modify the theorem:
+ parametrize C HMAC by OPAD and IPAD + they need to be different in at least one bit
+   (email adam: does he use this in his proof?)
 
-Lennart: update spec, ipad and opad
-email andrew about lennart coming to meeting + hmac refactoring
+Now, write individual functions and prove them equivalent? they have different types
+Still abstract: sha_h, sha_splitandpad, fpad?
 
+Figure out what lemmas to prove (Look in HMAC_Lemmas)
+
+Lennart: update spec to take ipad and opad as parameters
  *)
+Check HMAC.
 
-Check sha_h.
-
+(* ------------------------------------- *)
 Module Equiv.
-Definition c := (8 * SHA256_.DigestLength)%nat.
-Variable p : nat.
-Check HMAC (sha_h c plus). 
-Check HMAC (sha_h c plus) sha_iv.
 
-(* c needs to be not forall, should be 8 * digest length *)
+Definition c:nat := (SHA256_.DigestLength * 8)%nat.
+(*Variable p:nat.
+Locate HMAC.
+Check @HMAC. Check @sha_h.
+Check (@HMAC _ p (@sha_h _ p plus) sha_iv (sha_splitandpad_vector p) (fpad p)). 
+Check (HMAC (sha_h p plus) sha_iv).
+*)
+Definition p:=(32 * 8)%nat.
+
+(* Define opad, define ipad, pass converted ipad/opad to respective hmacs *)
+
+(* Is this the theorem we want? Is it useful for the rest of the proofs?
+Should it be more abstract? *)
+
+(* TODO: opad <> ipad? *)
+(* TODO fill this in *)
+Parameter bytes_bits_conv_vector' : byte -> Bvector (plus c p) -> Prop.
+
 Theorem HMAC_spec_equiv : forall
-                            (c p : nat)
                             (k m h : list Z)
-                            (K : Bvector (plus c p)) (M : Blist) (H : Bvector c),
-                            
-                            (* assuming k is already padded? *)
-  (8 * (length (HMAC_FUN.mkKey k)))%nat = (c + p)%nat ->
-  bytes_bits_vector c p k K -> bytes_bits_lists m M ->
-  HMAC (sha_h c plus) sha_iv (sha_splitandpad_vector c p) (fpad p) opad ipad K M = H ->
-  HMAC_FUN.HMAC k m = h ->
-  (* TODO fix HMAC h iv splitAndPad fpad opad ipad K M *)
+                            (K : Bvector (plus c p)) (M : Blist) (H : Bvector c)
+                            (op ip : byte) (OP IP : Bvector (plus c p)),
+  ((length k) * 8)%nat = b c p ->
+  bytes_bits_vector' k K ->
+  (* 1. not separating c and p 2. inductive prop / dep types? 3. computation / dep types?
+     bytes_bits_vector' k K vs. bytes_to_bits k = K <- can't prove lens equal?*)
+  bytes_bits_lists m M ->
+  bytes_bits_conv_vector' op OP ->
+  bytes_bits_conv_vector' ip IP ->
+  HMAC (sha_h p plus) sha_iv (sha_splitandpad_vector p) (fpad p) OP IP K M = H ->
+  HMAC_SHA256.HMAC op ip m k = h -> (* m k, not k m *)
   bytes_bits_vector' h H.
-Proof.
+Proof.  
+  intros k m h K M H op ip OP IP.
+  intros padded_key_len padded_keys_eq msgs_eq ops_eq ips_eq.
+  intros HMAC_abstract HMAC_concrete.
+  unfold p,c, b in *.
+  simpl in *.
+
+  unfold HMAC in *.
+  unfold HMAC_SHA256.HMAC in *.
+
+  unfold HMAC_2K in *. unfold GHMAC_2K in *. (* unfold splitVector in *. *)
+  (* Still abstract: sha_h, sha_splitandpad_vector, fpad *)
+
+  unfold HMAC_SHA256.OUTER in *. unfold HMAC_SHA256.INNER in *.
+    unfold HMAC_SHA256.outerArg in *. unfold HMAC_SHA256.innerArg in *.
+
+  rewrite <- HMAC_abstract.
+  rewrite <- HMAC_concrete.
+
 
 Abort.
-
