old/HMAC_functional_prog.v
@@ -2,39 +2,40 @@ Require Import Integers.
 Require Import Coqlib.
 Require Import Coq.Strings.String.
 Require Import Coq.Strings.Ascii.
-Require Import List. Import ListNotations.
+Require Import List. 
+
+Require Import sha.SHA256.
+Require Import sha.functional_prog.
+Notation "[ ]" := nil.
+Notation "[ x , .. , y ]" := (cons x .. (cons y []) ..).
 
 (*SHA256: blocksize = 64bytes 
     corresponds to 
     #define SHA_LBLOCK	16
     #define SHA256_CBLOCK	(SHA_LBLOCK*4) *)
 
-Module Type HASH_FUNCTION.
-  Parameter BlockSize:nat. (*measured in bytes; 64 in SHA256*)
-  Parameter DigestLength: nat. (*measured in bytes; 32 in SHA256*)
-  Parameter Hash : list Z -> list Z.
-End HASH_FUNCTION.
-
-
-Module Type HMAC_Module.
-  Parameter HMAC: byte -> byte -> list Z -> list Z -> list Z.
-End HMAC_Module.
-
-Module HMAC_FUN (HF:HASH_FUNCTION)  <: HMAC_Module.
 Fixpoint Nlist {A} (i:A) n: list A:=
   match n with O => nil
   | S m => i :: Nlist i m
   end.
 
-Definition sixtyfour {A} (i:A): list A:= Nlist i HF.BlockSize.
+Definition sixtyfour {A} (i:A): list A:= Nlist i 64%nat.
+
+Definition SHA256_DIGEST_LENGTH := 32.
+Definition SHA256_BlockSize := 64%nat.
+
+Definition Ipad := Byte.repr 54. (*0x36*)
+Definition Opad := Byte.repr 92. (*0x5c*)
+
+Module HMAC_FUN.
 
 (*Reading rfc4231 reveals that padding happens on the right*)
 Definition zeroPad (k: list Z) : list Z :=
-  k ++ Nlist Z0 (HF.BlockSize-length k).
+  k ++ Nlist Z0 (SHA256_BlockSize-length k).
 
 Definition mkKey (l:list Z) : list Z :=
-  if Z.gtb (Zlength l) (Z.of_nat HF.BlockSize)
-  then (zeroPad (HF.Hash l)) 
+  if Z.gtb (Zlength l) (Z.of_nat SHA256_BlockSize)
+  then (zeroPad (SHA_256' l)) 
   else zeroPad l.
 
 Definition mkArg (key:list byte) (pad:byte): list byte := 
@@ -42,48 +43,27 @@ Definition mkArg (key:list byte) (pad:byte): list byte :=
           (combine key (sixtyfour pad))).
 Definition mkArgZ key (pad:byte): list Z := 
      map Byte.unsigned (mkArg key pad).
-(*
-Definition Ipad := P.Ipad.  
-Definition Opad := P.Opad.
-*)
+
 (*innerArg to be applied to message, (map Byte.repr (mkKey password)))*)
-Definition innerArg IP (text: list Z) key : list Z :=
-  (mkArgZ key IP) ++ text.
+Definition innerArg (text: list Z) key : list Z :=
+  (mkArgZ key Ipad) ++ text.
 
-Definition INNER IP k text := HF.Hash (innerArg IP text k).
+Definition INNER k text := SHA_256' (innerArg text k).
 
-Definition outerArg OP (innerRes: list Z) key: list Z :=
-  (mkArgZ key OP) ++ innerRes.
+Definition outerArg (innerRes: list Z) key: list Z :=
+  (mkArgZ key Opad) ++ innerRes.
 
-Definition OUTER OP k innerRes := HF.Hash (outerArg OP innerRes k).
+Definition OUTER k innerRes := SHA_256' (outerArg innerRes k).
 
-Definition HMAC IP OP txt password: list Z := 
+Definition HMAC txt password: list Z := 
   let key := map Byte.repr (mkKey password) in
-  OUTER OP key (INNER IP key txt).
-
-End HMAC_FUN.
-
-Require Import SHA256.
-Require Import functional_prog.
-
-Module SHA256_ <: HASH_FUNCTION.
-  Definition BlockSize:= 64%nat.
-  Definition DigestLength:= 32%nat.
-  Definition Hash : list Z -> list Z := SHA_256'.
-End SHA256_.
-
-Module HMAC_SHA256 := HMAC_FUN SHA256_.
-
-Definition Ipad := Byte.repr 54. (*0x36*) 
-Definition Opad := Byte.repr 92. (*0x5c*)
-
-Definition HMAC256 := HMAC_SHA256.HMAC Ipad Opad.
+  OUTER key (INNER key txt).
 
 Definition HMACString (txt passwd:string): list Z :=
-  HMAC256 (str_to_Z txt) (str_to_Z passwd).
+  HMAC (str_to_Z txt) (str_to_Z passwd).
 
 Definition HMACHex (text password:string): list Z := 
-  HMAC256 (hexstring_to_Zlist text) (hexstring_to_Zlist password).
+  HMAC (hexstring_to_Zlist text) (hexstring_to_Zlist password).
 
 Definition check password text digest := 
   listZ_eq (HMACString text password) (hexstring_to_Zlist digest) = true.
@@ -121,3 +101,5 @@ Lemma RFC6868_exampleAUTH256_2:
   "7768617420646f2079612077616e7420666f72206e6f7468696e673f"
   "167f928588c5cc2eef8e3093caa0e87c9ff566a14794aa61648d81621a2a40c6".
 vm_compute. reflexivity. Qed.
+
+End HMAC_FUN.
