old/HMAC_lemmas_old.v
@@ -1,4 +1,4 @@
-Require Import floyd.proofauto. (* TODO *)
+Require Import floyd.proofauto.
 
 Import ListNotations.
 Local Open Scope logic.
@@ -6,16 +6,6 @@ Require Import sha.SHA256.
 Require Import sha.spec_sha.
 Require Import sha_lemmas.
 Require Import sha.HMAC_functional_prog.
-
-Lemma skipn_app2:
- forall A n (al bl: list A),
-  (n >= length al)%nat ->
-  skipn n (al++bl) = skipn (n-length al) bl.
-Proof.
-intros. revert al H;
-induction n; destruct al; intros; simpl in *; try omega; auto.
-apply IHn; omega.
-Qed. 
 
 Lemma firstn_app1: forall {A} n (p l: list A),
   (n <= Datatypes.length p)%nat ->
@@ -61,34 +51,33 @@ Proof. intros n.
     rewrite IHn; trivial. inversion H; trivial.
 Qed. 
 
+
+
 Lemma first64_sixtyfour {A} (a:A): 
-      firstn 64 (HMAC_SHA256.sixtyfour a) = HMAC_SHA256.sixtyfour a.
+      firstn 64 (sixtyfour a) = sixtyfour a.
 Proof. apply firstn_precise. simpl. reflexivity. Qed. 
 
-Lemma length_Nlist {A} (i:A): forall n, length (HMAC_SHA256.Nlist i n) = n.
+Lemma length_Nlist {A} (i:A): forall n, length (Nlist i n) = n.
 Proof. induction n; simpl; auto. Qed.
-
-Lemma length_SF {A} (x:A): length (HMAC_SHA256.sixtyfour x) = 64%nat.
-Proof. unfold HMAC_SHA256.sixtyfour. rewrite length_Nlist; trivial. Qed.
 
 Lemma str_to_Z_length: forall k, 
       String.length k = length (str_to_Z k).
 Proof. intros. induction k; simpl; auto. Qed.
   
-Lemma Zlength_mkArgZ k pad: Zlength (HMAC_SHA256.mkArgZ k pad) = Z.of_nat (min (length k) 64).
+Lemma Zlength_mkArgZ k pad: Zlength (HMAC_FUN.mkArgZ k pad) = Z.of_nat (min (length k) 64).
 Proof. intros. repeat rewrite Zlength_correct.
-   unfold HMAC_SHA256.mkArgZ, HMAC_SHA256.mkArg, HMAC_SHA256.sixtyfour.
+   unfold HMAC_FUN.mkArgZ, HMAC_FUN.mkArg, sixtyfour.
    repeat rewrite map_length. 
    rewrite combine_length, length_Nlist. trivial.
 Qed. 
 
-Lemma In_Nlist {A:Type}: forall (n:A) l x, In x (HMAC_SHA256.Nlist n l) -> x=n.
+Lemma In_Nlist {A:Type}: forall (n:A) l x, In x (Nlist n l) -> x=n.
 Proof. intros n l.
   induction l; simpl; intros. contradiction.
   destruct H; eauto.
 Qed.
-Lemma zeropad_isbyteZ: forall l, Forall isbyteZ l -> Forall isbyteZ (HMAC_SHA256.zeroPad l).
-Proof. unfold isbyteZ, HMAC_SHA256.zeroPad; intros.
+Lemma zeropad_isbyteZ: forall l, Forall isbyteZ l -> Forall isbyteZ (HMAC_FUN.zeroPad l).
+Proof. unfold isbyteZ, HMAC_FUN.zeroPad; intros.
   rewrite Forall_forall in *. intros.
   apply in_app_or in H0.
   destruct H0. apply (H _ H0).
@@ -97,23 +86,16 @@ Qed.
 Lemma mapnth': forall {A B : Type} (f : A -> B) (l : list A) (d : A) (n : nat) fd,
       fd = f d -> nth n (map f l) fd = f (nth n l d).
 Proof. intros; subst. apply map_nth. Qed.
-
-Lemma unsigned_Brepr_isbyte z: isbyteZ z -> Byte.unsigned (Byte.repr z) = z.
-Proof. intros. 
-      unfold isbyteZ in H. apply Byte.unsigned_repr.
-      unfold Byte.max_unsigned, Byte.modulus. simpl. omega.
-Qed.  
-
 Lemma map_unsigned_Brepr_isbyte: forall l, Forall isbyteZ l ->
       map Byte.unsigned (map Byte.repr l) = l.
 Proof. intros. induction l; simpl in *. trivial.
-   rewrite IHl. rewrite Forall_forall in H. 
+   rewrite IHl. rewrite Byte.unsigned_repr. trivial. 
+   rewrite Forall_forall in H. 
    assert (In a (a::l)). left. trivial. 
    specialize (H _ H0); clear H0.
-   rewrite unsigned_Brepr_isbyte; trivial.
+      unfold isbyteZ in H. unfold Byte.max_unsigned, Byte.modulus. simpl. omega.
    rewrite Forall_forall in *. intros. apply H. right; trivial.
 Qed.
-
 Lemma Ztest_Bytetest:
  forall a, Z.testbit (Byte.unsigned a) = Byte.testbit a.
 Proof. reflexivity. Qed.
@@ -172,7 +154,7 @@ apply H0.
 Qed.
 
 Lemma nth_Nlist {A}: forall (a d:A) k i (Hik: (i <k)%nat),
-      nth i (HMAC_SHA256.Nlist a k) d = a.
+      nth i (Nlist a k) d = a.
 Proof. intros a d k.
   induction k; simpl. 
     intros. omega.
@@ -181,7 +163,7 @@ Proof. intros a d k.
 Qed. 
 
 Lemma map_Nlist: forall {A B} a (f:A -> B) n,
-                 map f (HMAC_SHA256.Nlist a n) = HMAC_SHA256.Nlist (f a) n.
+                 map f (Nlist a n) = Nlist (f a) n.
 Proof. intros. induction n; simpl; trivial. rewrite IHn. trivial. Qed.
 
 Lemma minus_lt_compat_r: forall n m p : nat,
@@ -215,8 +197,8 @@ Proof.
 Qed.
 
 Lemma nth_zeropad_left {d d'}: forall l i (I: 0<= i < Zlength l),
-      nth (Z.to_nat i) (HMAC_SHA256.zeroPad l) d = nth (Z.to_nat i) l d'.
-Proof. unfold HMAC_SHA256.zeroPad. intros.
+      nth (Z.to_nat i) (HMAC_FUN.zeroPad l) d = nth (Z.to_nat i) l d'.
+Proof. unfold HMAC_FUN.zeroPad. intros.
   destruct I.
   apply Z2Nat.inj_lt in H0; try omega.
   rewrite Zlength_correct, Nat2Z.id in H0.
@@ -226,14 +208,14 @@ Qed.
 
 Lemma mkKey_left {d d'}: forall l (L: false = (Zlength l >? 64)) 
         i (I: 0<= i < Zlength l),
-      nth (Z.to_nat i) (HMAC_SHA256.mkKey l) d = nth (Z.to_nat i) l d'.
+      nth (Z.to_nat i) (HMAC_FUN.mkKey l) d = nth (Z.to_nat i) l d'.
 Proof.
-  unfold HMAC_SHA256.mkKey. intros. simpl. rewrite <- L.
+  unfold HMAC_FUN.mkKey. intros. simpl. rewrite <- L.
   apply nth_zeropad_left; trivial.
 Qed.
 Lemma nth_zeropad_right {d}: forall l i (I: Zlength l <= i < 64),
-      nth (Z.to_nat i) (HMAC_SHA256.zeroPad l) d = Z0.
-Proof. unfold HMAC_SHA256.zeroPad. intros.
+      nth (Z.to_nat i) (HMAC_FUN.zeroPad l) d = Z0.
+Proof. unfold HMAC_FUN.zeroPad. intros.
   rewrite app_nth2. rewrite nth_Nlist. trivial.
   apply minus_lt_compat_r. destruct I. apply Z2Nat.inj_lt in H0. apply H0.
   specialize (initial_world.zlength_nonneg _ l). omega.
@@ -247,9 +229,9 @@ Proof. unfold HMAC_SHA256.zeroPad. intros.
 Qed.
 Lemma mkKey_right {d}: forall l (L: false = (Zlength l >? 64)) 
         i (I: Zlength l <= i < 64),
-      nth (Z.to_nat i) (HMAC_SHA256.mkKey l) d = Z0.
+      nth (Z.to_nat i) (HMAC_FUN.mkKey l) d = Z0.
 Proof.
-  unfold HMAC_SHA256.mkKey. intros. simpl. rewrite <- L.
+  unfold HMAC_FUN.mkKey. intros. simpl. rewrite <- L.
   apply nth_zeropad_right; trivial.
 Qed.
 
@@ -369,52 +351,34 @@ Proof.
   intros. subst. apply offset_val_array_at0; trivial.
 Qed.
 
-Lemma split_memory_block p hi v sh:
-      0 <= p <= hi -> isptr v ->
-      memory_block sh (Int.repr hi) v =
-      !!offset_in_range (sizeof tuchar * 0) v &&
-      !!offset_in_range (sizeof tuchar * hi) v &&
-      memory_block sh (Int.repr p) v * memory_block sh (Int.repr (hi-p)) (offset_val (Int.repr p) v).
-Proof. intros.
-rewrite memory_block_array_tuchar'; try omega; trivial. 
-rewrite memory_block_array_tuchar'; try omega; trivial. 
-rewrite memory_block_array_tuchar'; try omega.   
-rewrite (split_offset_array_at_ _ _ _ p).
-   assert (K: (sizeof tuchar * p = p)%Z).
-      assert (sizeof tuchar =1 ). reflexivity.
-  rewrite H1. omega.
-  rewrite K; trivial.
- assumption. simpl; omega. reflexivity. apply isptr_offset_val'; trivial.
-Qed.
-
-Lemma zeroPad_BlockSize: forall k, (length k <= SHA256.BlockSize)%nat ->
-  length (HMAC_SHA256.zeroPad k) = SHA256.BlockSize%nat.
-Proof. unfold HMAC_SHA256.zeroPad. intros. rewrite app_length, length_Nlist. omega. 
+Lemma zeroPad_BlockSize: forall k, (length k <= SHA256_BlockSize)%nat ->
+  length (HMAC_FUN.zeroPad k) = SHA256_BlockSize%nat.
+Proof. unfold HMAC_FUN.zeroPad. intros. rewrite app_length, length_Nlist. omega. 
 Qed. 
 
 Lemma length_SHA256': forall l, 
-  length (functional_prog.SHA_256' l) = SHA256.DigestLength.
+  length (functional_prog.SHA_256' l) = Z.to_nat SHA256_DIGEST_LENGTH.
 Proof. intros. unfold functional_prog.SHA_256'. simpl.
   rewrite length_intlist_to_Zlist, functional_prog.length_process_msg. reflexivity.
 Qed.
  
-Lemma mkKey_length l: length (HMAC_SHA256.mkKey l) = SHA256.BlockSize.
-Proof. intros. unfold HMAC_SHA256.mkKey.
-  remember (Zlength l >? Z.of_nat SHA256.BlockSize) as z. 
+Lemma mkKey_length l: length (HMAC_FUN.mkKey l) = SHA256_BlockSize.
+Proof. intros. unfold HMAC_FUN.mkKey.
+  remember (Zlength l >? Z.of_nat SHA256_BlockSize) as z. 
   destruct z. apply zeroPad_BlockSize.
     rewrite length_SHA256'.  
     apply Nat2Z.inj_le. simpl. omega. 
   apply zeroPad_BlockSize.
     rewrite Zlength_correct in Heqz. 
     apply Nat2Z.inj_le. 
-    specialize (Zgt_cases (Z.of_nat (Datatypes.length l)) (Z.of_nat SHA256.BlockSize)). rewrite <- Heqz. trivial.
+    specialize (Zgt_cases (Z.of_nat (Datatypes.length l)) (Z.of_nat SHA256_BlockSize)). rewrite <- Heqz. trivial.
 Qed.
 
-Lemma mkKey_atBlockSize s: length s = SHA256.BlockSize%nat ->
-      HMAC_SHA256.mkKey s = s.
-Proof. unfold HMAC_SHA256.mkKey. rewrite Zlength_correct.
+Lemma mkKey_atBlockSize s: length s = SHA256_BlockSize%nat ->
+      HMAC_FUN.mkKey s = s.
+Proof. unfold HMAC_FUN.mkKey. rewrite Zlength_correct.
   intros. rewrite H.
-  simpl. unfold HMAC_SHA256.zeroPad. rewrite H. simpl.
+  simpl. unfold HMAC_FUN.zeroPad. rewrite H. simpl.
   apply app_nil_r.  
 Qed.
 
@@ -441,20 +405,4 @@ Proof. intros. inversion H; clear H.
               rewrite Zlength_app, Zlength_intlist_to_Zlist.
               rewrite (Z.mul_comm WORD). rewrite Z.mul_add_distr_r. trivial. 
   rewrite H; trivial.
-Qed.
-
-Lemma Zlength_max_zero: forall {A:Type} (l:list A), Z.max 0 (Zlength l) = Zlength l.
-Proof. intros.
-       rewrite Z.max_r. trivial.  
-       apply (initial_world.zlength_nonneg _ l).
-Qed.
-
-Lemma HMAC_length d k: length (HMAC_SHA256.HMAC d k) = 32%nat.
-Proof.
-  unfold HMAC_SHA256.HMAC, HMAC_SHA256.OUTER.
-  apply length_SHA256'.
-Qed.
-Lemma HMAC_Zlength d k: Zlength (HMAC_SHA256.HMAC d k) = 32.
-Proof.
-  rewrite Zlength_correct, HMAC_length. reflexivity.
 Qed.
